## P3-1
(a)
$$x_1 = y, x_2 = \dot{y}$$

(b)
$$m\dot{x_2} = F(t) - bx_2 - kx_1$$

(c)
$$\frac{d}{dt}x(t) = \left(\begin{array}{cc} 0 & 1\\\ -\frac{k}{m} & -\frac{b}{m} \end{array}\right)x(t)+ \left(\begin{array}{c} 0\\\ \frac{1}{m} \end{array}\right)F(t)$$


## P3-3
$$\frac{d}{dt}x(t) =\left(\begin{array}{cc} 0 & \frac{1}{L}\\\ -\frac{1}{C} & -\frac{1}{CR} \end{array}\right)x(t)+\left(\begin{array}{cc} -\frac{1}{L} & -\frac{1}{L}\\\ 0 & \frac{1}{CR} \end{array}\right)\left(\begin{array}{c} v_1\\\ v_2 \end{array}\right)
$$


## P3-5
$$\frac{s+2}{s\,\left(\frac{s+2}{s\,\left(s-3\right)\,\left(s+8\right)}+1\right)\,\left(s-3\right)\,\left(s+8\right)}$$


## P3-12



## P3-17


